First pass at completing proof

theories/Test.v
@@ -1,6 +1,5 @@
 Require Import Unicode.Utf8.
 Require Import Relations.Relation_Operators.
-(* Require Import Program.Equality List Lia. *)
 Require Import List.
 Require Import Autosubst.Autosubst.
 
@@ -50,6 +49,13 @@ Definition multistep := clos_refl_trans_1n _ step.
 Notation "e '-->*' e'" := (multistep e e') (at level 80).
 #[export] Hint Constructors clos_refl_trans_1n : core.
 
+Lemma multistep_step : ∀ x y, x --> y → x -->* y.
+Proof.
+  intros. econstructor; eauto.
+Qed.
+
+#[export] Hint Resolve multistep_step : core.
+
 Lemma multistep_trans : ∀ x y z, x -->* y → y -->* z → x -->* z.
 Proof.
   intros x y z H.
@@ -87,6 +93,13 @@ Section Examples.
 
 End Examples.
 
+Definition irred (e : term) := forall e', ¬ (e --> e').
+Ltac irred_step :=
+  match goal with
+  | [ H : irred ?e, Hstep : ?e --> ?e' |- _ ] => exfalso; apply H in Hstep; assumption
+  end.
+
+
 Section Deterministic.
   Theorem step_deterministic : ∀ {s t₁ t₂ : term},
       s --> t₁ →
@@ -122,11 +135,6 @@ Section Deterministic.
         apply IHHu. apply Hv.
   Qed.
 
-  Definition irred (e : term) := forall e', ¬ (e --> e').
-  Ltac irred_step :=
-    match goal with
-    | [ H : irred ?e, Hstep : ?e --> ?e' |- _ ] => exfalso; apply H in Hstep; assumption
-    end.
 
   Corollary irred_unique : ∀ a b c, a -->* b → a -->* c → irred b → c -->* b.
   Proof.
@@ -186,18 +194,8 @@ Section TypeSafety.
   | sem_exprC : ∀ τ e, (∀ e', e -->* e' → (* irred(e') → *) sem_value τ e') → sem_expr τ e.
   *)
 
-
-  Axiom LEM : ∀ P, P ∨ ¬ P.
   Lemma irred_decidable : ∀ e, (∃ e', e --> e') ∨ irred e.
   Proof.
-    intros e.
-    destruct (LEM (∃ e', e --> e')); auto.
-    right.
-    intros e' Hstep.
-    eauto.
-  Qed.
-
-  (*
     induction e.
     - right. intros e' H. value_step.
     - right. intros e' H. value_step.
@@ -213,11 +211,15 @@ Section TypeSafety.
       destruct (value_dec e1).
       * left. eexists. apply step_app2. apply H1. apply H0.
       * right. intros e' Hstep. inversion Hstep; subst. value_step. irred_step. apply H1. assumption.
-
       * destruct (value_dec e1).
-        destruct (value_dec e2).
-  Admitted. *)
-
+        destruct H1.
+        + right. intros e' Hstep. inversion Hstep; subst. irred_step. irred_step.
+        + right. intros e' Hstep. inversion Hstep; subst. irred_step. irred_step.
+        + destruct (value_dec e2).
+          ++ left. exists e.[e2/]. constructor; auto.
+          ++ right. intros e' Hstep. inversion Hstep; subst. auto. inversion H5. irred_step.
+        + right. intros e' Hstep. inversion Hstep; subst. apply H1. constructor. irred_step. irred_step.
+  Qed.
 
   (* The easiest way to write this is to avoid mutual recursion altogether, since Coq's termination checker isn't smart enough to see that this is well-founded. *)
   Fixpoint sem_value (T : type) : term → Prop :=
@@ -285,6 +287,38 @@ Section TypeSafety.
       auto.
   Qed.
 
+
+  (* Need a bunch of congruence step lemmas: *)
+  Lemma if_cond_step : ∀ e1 e2 e3 e1', e1 -->* e1' → TIf e1 e2 e3 -->* TIf e1' e2 e3.
+  Proof.
+    intros.
+    induction H; auto.
+    constructor.
+    econstructor.
+    constructor. apply H.
+    assumption.
+  Qed.
+
+  Lemma app_cong1 : ∀ e1 e2 e1', e1 -->* e1' → TApp e1 e2 -->* TApp e1' e2.
+  Proof.
+    intros.
+    induction H.
+    constructor.
+    econstructor.
+    constructor. apply H.
+    assumption.
+  Qed.
+
+  Lemma app_cong2 : ∀ τ e1 e2 e2', e2 -->* e2' → TApp (TLam τ e1) e2 -->* TApp (TLam τ e1) e2'.
+  Proof.
+    intros.
+    induction H.
+    constructor.
+    econstructor.
+    apply step_app2. constructor. apply H.
+    assumption.
+  Qed.
+
   (* When If takes a step, either we take a step to another If, or we step to one of the branches.
    If the whole expression steps to a reducible value, e1 must have stepped to a reducible value.
    The induction principle is tricky, naively inducting on the Hif doesn't seem to work. Instead we write it using a fixpoint, but we need to be careful to ensure the arguments are decreasing. *)
@@ -308,19 +342,46 @@ Section TypeSafety.
       * exists e1. split. constructor. auto.
    Qed.
 
-  Print tif_lemma.
-
-  (* Need a bunch of congruence step lemmas: *)
-  Lemma if_cond_step : ∀ e1 e2 e3 e1', e1 -->* e1' → TIf e1 e2 e3 -->* TIf e1' e2 e3.
+  Fixpoint app_lemma1 {e1 e2 e' : term} (He' : irred e') (H : TApp e1 e2 -->* e') : ∃ e1', e1 -->* e1' ∧ irred e1'.
   Proof.
-    intros.
-    induction H; auto.
-    constructor.
-    econstructor.
-    constructor. apply H.
-    assumption.
+    destruct H.
+    - exists e1. split. constructor.
+      intros e1' Hstep.
+      assert (TApp e1 e2 --> TApp e1' e2). constructor; auto.
+      unfold irred in He'. specialize He' with (TApp e1' e2). auto.
+    - destruct (irred_decidable e1).
+      * destruct H1 as [e1' ?]. specialize app_lemma1 with e1' e2 z.
+        apply app_lemma1 in He'.
+        destruct He' as [e1'' [? ?]].
+        exists e1''. split.
+        econstructor. apply H1. apply H2.
+        assumption.
+        assert (TApp e1 e2 --> TApp e1' e2). constructor. auto.
+        assert (y = TApp e1' e2). apply (step_deterministic H H2).
+        rewrite H3 in *. apply H0.
+      * exists e1. split. constructor. auto.
   Qed.
 
+  Fixpoint app_lemma2 {τ} {e e2 e' : term} (He' : irred e') (H : TApp (TLam τ e) e2 -->* e') {struct H} : ∃ e2', e2 -->* e2' ∧ irred e2'.
+  Proof.
+    destruct H.
+    - exists e2. split. constructor.
+      intros e2' Hstep.
+      assert (TApp (TLam τ e) e2 --> TApp (TLam τ e) e2'). apply step_app2; auto.
+      unfold irred in He'. specialize He' with (TApp (TLam τ e) e2'). auto.
+    - destruct (irred_decidable e2).
+      * destruct H1 as [e2' ?]. specialize app_lemma2 with τ e e2' z.
+        apply app_lemma2 in He'.
+        destruct He' as [e2'' [? ?]].
+        exists e2''. split.
+        + econstructor. apply H1. assumption.
+        + assumption.
+        + assert (TApp (TLam τ e) e2 --> TApp (TLam τ e) e2'). apply step_app2; auto.
+          assert (y = TApp (TLam τ e) e2'). apply (step_deterministic H H2).
+          rewrite H3 in *.
+          assumption.
+      * exists e2. split. constructor. auto.
+  Qed.
 
   Lemma fund_lemma : ∀ e τ, ⊢ e ∈ τ → ⊧ e ∈ τ.
   Proof.
@@ -347,13 +408,37 @@ Section TypeSafety.
     - (* App case *) unfold sem_has_type in IHHe1, IHHe2.
       specialize IHHe1 with γ.
       specialize IHHe2 with γ.
-      admit.
+      unfold sem_expr in IHHe1.
+      intros e' Hstep He'.
+      destruct (app_lemma1 He' Hstep) as [f' [? ?]].
+      assert (TApp f.[γ] e.[γ] -->* TApp f' e.[γ]). { apply app_cong1; auto. }
+      specialize IHHe1 with f'.
+      rewrite sem_value_arr in IHHe1.
+      destruct IHHe1 as [f'' [? ?]]; auto.
+      subst.
+      destruct (app_lemma1 He' Hstep) as [f' [? ?]].
+      assert (TApp (TLam τ₂ f'') e.[γ] -->* e'). {
+        eapply irred_unique. apply Hstep. assumption. assumption. }
+      destruct (app_lemma2 He' H5) as [e2' [? ?]].
+      unfold sem_expr in IHHe2.
+      specialize IHHe2 with e2'.
+
+      assert (e2' ∈ 𝓥⟦ τ₂ ⟧). { apply IHHe2; auto. }
+      assert (value e2'). { eapply sem_value_is_value; eauto. }
+      assert (TApp (TLam τ₂ f'') e.[γ] -->* TApp (TLam τ₂ f'') e2'). { apply app_cong2; auto. }
+      assert (TApp (TLam τ₂ f'') e2' -->* f''.[e2'/]). { econstructor; auto. }
+      assert (f''.[e2'/] ∈ 𝓔⟦ τ ⟧). { apply H3. auto. }
+      assert (f''.[e2'/] -->* e').
+      { eapply irred_unique; eauto.
+        apply Operators_Properties.clos_rt_rt1n_iff.
+        eapply rt_trans.
+        apply Operators_Properties.clos_rt_rt1n_iff. apply H10.
+        apply Operators_Properties.clos_rt_rt1n_iff. apply H11. }
+      apply H12; auto.
     - (* If case *) unfold sem_has_type in IHHe1, IHHe2, IHHe3.
       specialize IHHe1 with γ.
       intros e' Hstep He'.
       unfold sem_expr in IHHe1.
-
-      (* Need this tif_lemma: *)
       destruct (tif_lemma _ _ _ He' _ Hstep) as [e1' [Hif1 Hif2]].
       assert (TIf e.[γ] e₁.[γ] e₂.[γ] -->*
                                     TIf e1' e₁.[γ] e₂.[γ]). { auto using if_cond_step. }
@@ -377,7 +462,7 @@ Section TypeSafety.
           apply H. econstructor. apply H0. auto. auto.
         }
         eapply IHHe3; eauto.
-  Admitted.
+  Qed.
 
   Lemma sem_type_implies_safe : ∀ e τ, ⊧ e ∈ τ → safe e.
   Proof.
@@ -392,6 +477,11 @@ Section TypeSafety.
     - left.
       eapply sem_value_is_value. apply H; auto.
   Qed.
+
+  Print sem_type_implies_safe.
+  Print Assumptions irred_decidable.
+
+  Print Assumptions sem_type_implies_safe.
 
   Theorem type_safety : ∀ τ t, ⊢ t ∈ τ → safe t.
   Proof.
